examples/ijr/examplesScript.sml
@@ -1,0 +1,37 @@
+open HolKernel Parse boolLib bossLib;
+
+open bslSyntax bir_execLib;
+
+open resolveTheory;
+
+val _ = new_theory "examples";
+
+
+val observe_type = Type `: 'a`
+val bdefprog_list = bdefprog_list observe_type
+
+val block1 = (blabel_addr32 0,
+              [bassign (bvarimm32 "y", bconst32 4)],
+              (bjmp o belabel_expr o bden o bvarimm32) "y")
+
+val block2: term * term list * term  = (blabel_addr32 4, [], (bhalt o bconst32) 0)
+
+val prog_def = bdefprog_list "prog" [block1, block2]
+val prog = (snd o dest_eq o concl) prog_def
+
+val n_max = 10;
+val _ = bir_exec_prog_print "prog" prog n_max NONE NONE NONE;
+
+val prog'_def = EVAL “resolve_fail ^prog (BL_Address (Imm32 0w))”
+val prog' = (dest_some o snd o dest_eq o concl) prog'_def
+
+val _ = bir_exec_prog_print "prog'" prog' n_max NONE NONE NONE;
+
+val prog'_def = EVAL “resolve ^prog (BL_Address (Imm32 0w)) (Imm32 10w) "fresh"”
+val prog' = (dest_some o snd o dest_eq o concl) prog'_def
+
+(*val _ = bir_exec_prog_print "prog'" prog' n_max NONE NONE NONE;*)
+
+
+val _ = export_theory();
+
